Update Sequent.thy

Sequent.thy
@@ -10,7 +10,7 @@ section \<open>Terms and formulae\<close>
 text \<open>
 \label{sec:terms} The datatypes of terms and formulae are defined as follows:
 \<close>
-datatype ('f) tm  = Var nat |  Fun 'f \<open>'f tm list\<close> 
+datatype ('f) tm  = Var nat | Fresh nat |  Fun 'f \<open>nat list\<close> 
 
 datatype sign = pos | neg
 
@@ -19,7 +19,6 @@ datatype ('f) form =
   | EqFresh sign "'f tm" "'f tm"
   | ConcEq "'f tm" "'f tm" "'f tm"
   | Member sign "'f tm" "char BA rexp"
-  | MemberFresh sign "'f tm" "char BA rexp"
   | Dis "'f form" "'f form"                     
   | Con "'f form" "'f form"                      
   | Neg "'f form"     
@@ -30,11 +29,11 @@ subsection \<open>Fresh term\<close>
 
 fun fresh_var :: "nat => 'f tm => bool" where
   "fresh_var x (Var y) = (x \<noteq> y)" |
-  "fresh_var x (Fun f xs) = (list_all (\<lambda>a. fresh_var x a) xs)" 
+  "fresh_var x (Fun f xs) = (list_all (\<lambda>a. a = x) xs)" 
 
 primrec deX :: "'f tm => nat list" where 
   "deX (Var n) = [n] "|
-  "deX (Fun f xs) = concat (map deX xs)"
+  "deX (Fun f xs) = xs"
 
 definition
   freshVar :: "string tm list => string tm" where
@@ -46,21 +45,19 @@ lemma "freshVar [Var (0::nat), Var 1, Var 3] = Var 2"
 
 subsection \<open>Semantics of term and form\<close>
 
-primrec semantics_tm and semantics_list where
-  \<open>semantics_tm e f (Var n) = e n\<close> |
-  \<open>semantics_tm e f (Fun i l) = f i (semantics_list e f l)\<close> |
-  \<open>semantics_list e f [] = []\<close> |
-  \<open>semantics_list e f (t # l) = semantics_tm e f t # semantics_list e f l\<close>
+primrec semantics_tm :: "(nat \<Rightarrow> string) \<Rightarrow> ('f \<Rightarrow> string list \<Rightarrow> string) \<Rightarrow> 'f tm \<Rightarrow> string" (\<open>\<lparr>_, _\<rparr>\<close>) where
+  \<open>\<lparr>E, F\<rparr> (Var n) = E n\<close> |
+  \<open>\<lparr>E, F\<rparr> (Fresh n) = E n\<close> |
+  \<open>\<lparr>E, F\<rparr> (Fun f ts) = F f (map E ts)\<close>
 
 fun concat_str :: "string \<Rightarrow> string list \<Rightarrow> string" where
   "concat_str s ls = (if s = ''concat'' then List.concat ls else [])"
 
 primrec semantics_fm (\<open>\<lbrakk>_, _\<rbrakk>\<close>) where
-  \<open>\<lbrakk>E, F\<rbrakk> (EqAtom s x y) = (if s = pos then semantics_tm E F x = semantics_tm E F y else semantics_tm E F x \<noteq> semantics_tm E F y)\<close> 
+  \<open>\<lbrakk>E, F\<rbrakk> (EqAtom s x y) = (if s = pos then \<lparr>E, F\<rparr> x = \<lparr>E, F\<rparr> y else \<lparr>E, F\<rparr> x \<noteq> \<lparr>E, F\<rparr> y)\<close> 
 | \<open>\<lbrakk>E, F\<rbrakk> (EqFresh s x y) = True\<close> 
-| \<open>\<lbrakk>E, F\<rbrakk> (ConcEq z x y) = (semantics_tm E F z = semantics_tm E F x @ semantics_tm E F y)\<close> 
-| \<open>\<lbrakk>E, F\<rbrakk> (Member s x r) = (if s = pos then semantics_tm E F x \<in> lang r else semantics_tm E F x \<notin> lang r)\<close> 
-| \<open>\<lbrakk>E, F\<rbrakk> (MemberFresh s x r) = True\<close> 
+| \<open>\<lbrakk>E, F\<rbrakk> (ConcEq z x y) = (\<lparr>E, F\<rparr> z = \<lparr>E, F\<rparr> x @ \<lparr>E, F\<rparr> y)\<close> 
+| \<open>\<lbrakk>E, F\<rbrakk> (Member s x r) = (if s = pos then \<lparr>E, F\<rparr> x \<in> lang r else \<lparr>E, F\<rparr> x \<notin> lang r)\<close> 
 | \<open>\<lbrakk>E, F\<rbrakk> (Dis x y) = (\<lbrakk>E, F\<rbrakk> x \<or> \<lbrakk>E, F\<rbrakk> y)\<close> 
 | \<open>\<lbrakk>E, F\<rbrakk> (Con x y) = (\<lbrakk>E, F\<rbrakk> x \<and> \<lbrakk>E, F\<rbrakk> y)\<close> 
 | \<open>\<lbrakk>E, F\<rbrakk> (Neg x) = (\<not> \<lbrakk>E, F\<rbrakk> x)\<close> 
@@ -88,9 +85,6 @@ fun exists_solution :: "string form list \<Rightarrow> bool" where
   "exists_solution ls = (if ls = [] then False 
                        else list_all is_Member ls \<and> distinct_variable ls \<and> single_word ls)"  
 
-definition model :: \<open>(nat \<Rightarrow> char list) \<Rightarrow> ('f \<Rightarrow> char list list \<Rightarrow> char list) \<Rightarrow> 'f form list \<Rightarrow> 'f form \<Rightarrow> bool\<close> ("_,_,_ \<Turnstile> _" [50,50] 50) where
-  \<open>(E,F,ps \<Turnstile> p) = (list_all \<lbrakk>E,F\<rbrakk> ps \<longrightarrow> \<lbrakk>E, F\<rbrakk> p)\<close>
-
 fun empty_intersection_set :: "char BA rexp list \<Rightarrow> bool" where
   "empty_intersection_set fs = (\<Inter>(lang ` set fs) = {} \<and> length fs > 1 )"
 
@@ -111,64 +105,64 @@ fun con_fwd_prop ::"char BA rexp \<Rightarrow> char BA rexp \<Rightarrow> char B
 fun con_fwd_prop_elim ::"char BA rexp \<Rightarrow> char BA rexp \<Rightarrow> char BA rexp \<Rightarrow> bool" where
   "con_fwd_prop_elim r e1 e2 = (lang r = lang (Times e1 e2) \<and> is_singleton (lang r))"
 
-primrec con_bwd_prop ::" char BA rexp \<Rightarrow> (char BA rexp * char BA rexp) set" where
-  "con_bwd_prop Zero = {(Zero, Zero)}"|
-  "con_bwd_prop 1\<^sub>r = {(One, One)}"|
-  "con_bwd_prop (Pred a) = {(Pred a, One), (One ,Pred a)}"|
-  "con_bwd_prop (Plus r1 r2) = {(Plus r1 r2, One), (One, Plus r1 r2)}"|
-  "con_bwd_prop (Times r1 r2) = {(r1, r2), (One ,Times r1 r2), (Times r1 r2, One)}"|
-  "con_bwd_prop (Inter r1 r2) = {(One ,Inter r1 r2), (Inter r1 r2, One)}"| (*FIXME: Not Enumerate*)
-  "con_bwd_prop (Star r) = {(Star r, Star r)}"
+fun con_bwd_prop ::" char BA rexp \<Rightarrow> (char BA rexp * char BA rexp) set" where
+  "con_bwd_prop r = {(a,b)|a b. lang r = (lang (Times a b))}"
 
-inductive One_SC :: \<open>string form list * string form list set \<Rightarrow> bool\<close> (\<open>\<stileturn> _\<close> 0) where
-  AlphaCon:      \<open>\<stileturn> ([Con A B] @ \<Gamma>, {[A,B] @ \<Gamma>})\<close>
-| AlphaNegOr:    \<open>\<stileturn> (Neg (Dis A B)# \<Gamma>, {Neg A #Neg B#\<Gamma>})\<close>
-| AlphaOr:       \<open>\<stileturn> ([Dis A B, \<Gamma>], {[A, \<Gamma>], [B, \<Gamma>]})\<close>
-| AlphaNegAnd:   \<open>\<stileturn> (Neg (Con A B) # \<Gamma>, {Neg A # \<Gamma>, Neg B # \<Gamma>})\<close>
-| AlphaNegNeg:   \<open>\<stileturn> (Neg (Neg A) # \<Gamma>, {A# \<Gamma>})\<close>
-| NotMember:     \<open>regexp_compl e ec \<Longrightarrow> \<stileturn> ((Member neg x e) # \<Gamma>, {(Member pos x ec) # \<Gamma>})\<close>
-| NotEq:         \<open>y = freshVar ([x,(Fun f xs)])  \<Longrightarrow> \<stileturn> ([EqAtom neg x (Fun f xs), \<Gamma>], {[EqFresh neg x y,  EqFresh pos y (Fun f xs), \<Gamma>]})\<close>
-| Cut:           \<open>regexp_compl e ec \<Longrightarrow> \<stileturn> (\<Gamma>, {Member pos x e # \<Gamma>, Member pos x ec # \<Gamma>})\<close>
-| EqProp:        \<open>\<stileturn> (Member pos x e # EqAtom pos x y # \<Gamma>, { Member pos x e # EqAtom pos x y # Member pos y e # \<Gamma>})\<close>
-| NeqSubsume:    \<open>regexp_empty e1 e2 \<Longrightarrow> \<stileturn> (Member pos x e1 # EqAtom neg x y # Member pos y e2 # \<Gamma>, {Member pos x e1 # Member pos y e2 # \<Gamma>})\<close>
-| EqPropElim:    \<open>is_singleton (lang e) \<Longrightarrow> \<stileturn> (Member pos x e # (EqAtom pos x y) # \<Gamma>, {Member pos x e # Member pos y e # \<Gamma>})\<close>
-| NeqPropElim:   \<open>is_singleton (lang e) \<Longrightarrow> regexp_compl e ec \<Longrightarrow> \<stileturn> ((Member pos x e) # (EqAtom neg x y) # \<Gamma>, {(Member pos x e) # (Member pos y ec) # \<Gamma>})\<close>
-| Close:         \<open>empty_intersection_set rs \<Longrightarrow> \<stileturn> (map (\<lambda>r. Member pos x r) rs, {})\<close> 
-| Subsume:       \<open>subset_intersect_set e fs \<Longrightarrow> \<stileturn> (Member pos x e # (map (\<lambda>r. Member pos x r) fs) @ \<Gamma>, {(map (\<lambda>r. Member pos x r) fs) @ \<Gamma>})\<close> 
-| Intersect:     \<open>eq_len_intersect e fs \<Longrightarrow> \<stileturn> ((map (\<lambda>r. Member pos x r) (fs)) @ \<Gamma>, {Member pos x e # \<Gamma>})\<close> 
-| Fwd_PropConc:  \<open>con_fwd_prop e e1 e2 \<Longrightarrow> \<stileturn> ([(EqAtom pos x (Fun ''concat'' [x1,x2])), (Member pos x1 e1), (Member pos x2 e2)] @ \<Gamma>, 
-{[(Member pos x e), (EqAtom pos x (Fun ''concat'' [x1,x2])), (Member pos x1 e1), (Member pos x2 e2)] @ \<Gamma>})\<close>  
+inductive One_SC :: \<open>string form list \<Rightarrow> bool\<close> (\<open>\<stileturn> _\<close> 0) where
+  AlphaCon:      \<open>\<stileturn> [A,B] @ \<Gamma> \<Longrightarrow> \<stileturn> [Con A B] @ \<Gamma>\<close>
+| AlphaNegOr:    \<open>\<stileturn> Neg A #Neg B#\<Gamma> \<Longrightarrow> \<stileturn> Neg (Dis A B)# \<Gamma>\<close>
+| AlphaOr:       \<open>\<stileturn> A# \<Gamma> \<Longrightarrow> \<stileturn> B# \<Gamma> \<Longrightarrow> \<stileturn> Dis A B # \<Gamma>\<close>
+| AlphaNegAnd:   \<open>\<stileturn> Neg A # \<Gamma> \<Longrightarrow>  \<stileturn> Neg B # \<Gamma> \<Longrightarrow> \<stileturn> Neg (Con A B) # \<Gamma>\<close>
+| AlphaNegNeg:   \<open>\<stileturn> A# \<Gamma> \<Longrightarrow> \<stileturn> Neg (Neg A) # \<Gamma>\<close>
+| NotMember:     \<open>regexp_compl e ec \<Longrightarrow> \<stileturn> (Member pos x ec) # \<Gamma> \<Longrightarrow> \<stileturn> (Member neg x e) # \<Gamma>\<close>
+| NotEq:         \<open>y = freshVar ([x,(Fun f xs)])  \<Longrightarrow> \<stileturn> [EqFresh neg x y,  EqFresh pos y (Fun f xs), \<Gamma>] \<Longrightarrow> \<stileturn> [EqAtom neg x (Fun f xs), \<Gamma>]\<close>
+| Cut:           \<open>regexp_compl e ec \<Longrightarrow> \<stileturn> Member pos x e # \<Gamma> \<Longrightarrow>  \<stileturn> Member pos x ec # \<Gamma> \<Longrightarrow>  \<stileturn> \<Gamma>\<close>
+| EqProp:        \<open>\<stileturn> Member pos x e # EqAtom pos x y # Member pos y e # \<Gamma> \<Longrightarrow> \<stileturn> Member pos x e # EqAtom pos x y # \<Gamma>\<close>
+| NeqSubsume:    \<open>regexp_empty e1 e2 \<Longrightarrow> \<stileturn> Member pos x e1 # Member pos y e2 # \<Gamma> \<Longrightarrow> \<stileturn> Member pos x e1 # EqAtom neg x y # Member pos y e2 # \<Gamma>\<close>
+| EqPropElim:    \<open>is_singleton (lang e) \<Longrightarrow> \<stileturn> Member pos x e # Member pos y e # \<Gamma>\<Longrightarrow> \<stileturn> Member pos x e # (EqAtom pos x y) # \<Gamma>\<close>
+| NeqPropElim:   \<open>is_singleton (lang e) \<Longrightarrow> regexp_compl e ec \<Longrightarrow> \<stileturn> (Member pos x e) # (Member pos y ec) # \<Gamma> \<Longrightarrow>  
+                 \<stileturn> (Member pos x e) # (EqAtom neg x y) # \<Gamma>\<close>
+| Close:         \<open>empty_intersection_set rs \<Longrightarrow> \<stileturn> map (\<lambda>r. Member pos x r) rs\<close> 
+| Subsume:       \<open>subset_intersect_set e fs \<Longrightarrow> \<stileturn> (map (\<lambda>r. Member pos x r) fs) @ \<Gamma> \<Longrightarrow> \<stileturn> Member pos x e # (map (\<lambda>r. Member pos x r) fs) @ \<Gamma>\<close> 
+| Intersect:     \<open>eq_len_intersect e fs \<Longrightarrow> \<stileturn> Member pos x e # \<Gamma>  \<Longrightarrow>  \<stileturn> (map (\<lambda>r. Member pos x r) (fs)) @ \<Gamma>\<close> 
+| Fwd_PropConc:  \<open>con_fwd_prop e e1 e2 \<Longrightarrow> \<stileturn> [(Member pos x e), (EqAtom pos x (Fun ''concat'' [x1,x2])), (Member pos (Var x1) e1), (Member pos (Var x2) e2)] @ \<Gamma>
+                 \<Longrightarrow> \<stileturn> [(EqAtom pos x (Fun ''concat'' [x1,x2])), (Member pos (Var x1) e1), (Member pos (Var x2) e2)] @ \<Gamma>\<close>  
+| Fwd_ElimConc:  \<open>con_fwd_prop_elim e e1 e2 \<Longrightarrow> \<stileturn> [Member pos x e, (Member pos (Var x1) e1), (Member pos (Var x2) e2)]  @ \<Gamma> \<Longrightarrow>  
+                 \<stileturn> [(EqAtom pos x (Fun ''concat'' [x1, x2])), (Member pos (Var x1) e1), (Member pos (Var x2) e2)] @ \<Gamma>\<close>
+(*| Bwd_PropConc:  \<open>con_bwd_prop e = es \<Longrightarrow> \<stileturn> ((\<lambda>r. [Member x e, EqAtom x (Fun ''concat'' [x1,x2]), Member (Var x1) (fst r), Member (Var x2) (snd r)] @ \<Gamma>) ` es) \<Longrightarrow> 
+                 \<stileturn> {[Member x e, EqAtom x (Fun ''concat'' [x1,x2])] @ \<Gamma>}\<close>*)
+| Order:         \<open>\<stileturn> G \<Longrightarrow> set G = set G' \<Longrightarrow> \<stileturn> G'\<close>
+| Basic:        \<open> \<stileturn> [A,Neg A, G]\<close>
+| BasicFF: \<open>\<stileturn> FF # G\<close>
 
-| Fwd_ElimConc:  \<open>con_fwd_prop_elim e e1 e2 \<Longrightarrow> \<stileturn> ([(EqAtom pos x (Fun ''concat'' [x1, x2])), (Member pos x1 e1), (Member pos x2 e2)] @ \<Gamma>,
-{ [Member pos x e, (Member pos x1 e1), (Member pos x2 e2)]  @ \<Gamma>})\<close>
-
-| Bwd_PropConc:  \<open>con_bwd_prop e \<noteq> {} \<Longrightarrow> \<stileturn> ([(EqAtom pos x (Fun ''concat'' [x1, x2])), (Member pos x e), \<Gamma>] ,
-(\<lambda>r. [Member pos x e, EqAtom pos x (Fun ''concat'' [x1, x2]), (MemberFresh pos x1 (fst r)), (MemberFresh pos x2 (snd r)), \<Gamma>]) ` con_bwd_prop e)\<close>
-| Order:         \<open>set G = set G' \<Longrightarrow> \<stileturn> (G', {G})\<close>
-| Basic:        \<open> \<stileturn> ([A,Neg A, G], {})\<close>
- 
 declare One_SC.intros [intro]
 
 subsection \<open>Soundness\<close>
 
-lemma SC_soundness: \<open>\<stileturn> G \<Longrightarrow> (\<forall>fs \<in> (snd G). \<exists>f \<in> set fs. \<not> \<lbrakk>E, concat_str\<rbrakk> f) \<Longrightarrow> (\<exists>p \<in> set (fst G). \<not> \<lbrakk>E, concat_str\<rbrakk> p) \<close>
-proof (induct rule: One_SC.induct)
-  case (NeqPropElim e ec x y \<Gamma>)
-  then show ?case apply auto 
-    by (metis (no_types, lifting) DiffI UNIV_I is_singletonE singletonD) 
-next
+lemma SC_soundness: \<open>\<stileturn> G \<Longrightarrow> (\<exists>p \<in> set G. \<not> \<lbrakk>E, concat_str\<rbrakk> p)\<close>
+proof (induct G rule: One_SC.induct)
   case (Intersect e fs x \<Gamma>)
-  then show ?case apply auto 
-    by (smt (verit, del_insts) INT_I image_subset_iff semantics_fm.simps(4) sup.cobounded1) 
+  then show ?case  apply auto 
+    by (smt (verit) INT_I image_subset_iff semantics_fm.simps(4) sup.cobounded1)
 qed (auto simp:l_prod_elim is_singleton_def)
+
+(*next
+  case (Bwd_PropConc e es x1 x2 x \<Gamma>)
+  then show ?case apply (auto simp:c_prod_def times_list_def) sorry*)
+
+definition SC_proof :: \<open>string form list \<Rightarrow> string form \<Rightarrow> bool\<close> where
+  \<open>SC_proof ps p \<equiv> (\<stileturn>  Neg p # ps)\<close>
+
+theorem sc_soundness:
+  \<open>SC_proof ps p \<Longrightarrow> list_all \<lbrakk>E, concat_str\<rbrakk> ps \<Longrightarrow> \<lbrakk>E, concat_str\<rbrakk> p\<close>
+  using SC_soundness unfolding SC_proof_def list_all_def
+  by fastforce
 
 subsection \<open>Consistent sets\<close>
 
-definition consistency :: \<open>string form set set \<Rightarrow> bool\<close> where
-  \<open>consistency C = (\<forall>S. S \<in> C \<longrightarrow> FF \<notin> S \<and> 
-               (\<forall>p q. \<not> (EqAtom pos p q \<in> S \<and> EqAtom neg  p q \<in> S) \<and>
-               \<not> (\<forall>x r. Member pos x r \<in> S \<and> Member pos x r \<in> S)) \<and> 
-              (\<forall> A B. Con A B \<in> S \<longrightarrow> S \<union> {A, B} \<in> C) \<and> 
+definition consistency :: "string form set set \<Rightarrow> bool" where
+  "consistency C = (\<forall>S. S \<in> C \<longrightarrow> FF \<notin> S \<and> 
+              (\<forall> A B. Con A B \<in> S \<longrightarrow> S \<union> {A, B} \<in> C) \<and>
               (\<forall> A B. Neg (Dis A B) \<in> S \<longrightarrow> S \<union> {Neg A, Neg B} \<in> C) \<and> 
               (\<forall> A B. Dis A B \<in> S \<longrightarrow> S \<union> {A} \<in> C \<or> S \<union> {B} \<in> C) \<and> 
               (\<forall> A B. Neg (Con A B) \<in> S \<longrightarrow> S \<union> {Neg A} \<in> C \<or> S \<union> {Neg B} \<in> C) \<and> 
@@ -183,15 +177,85 @@ definition consistency :: \<open>string form set set \<Rightarrow> bool\<close> 
               (\<forall> x rs. empty_intersection_set rs \<longrightarrow> S \<union> ((\<lambda>r. Member pos x r) ` (set rs)) \<in> C \<longrightarrow> S \<union> {FF} \<in> C) \<and> 
               (\<forall> x e fs. subset_intersect_set e fs \<longrightarrow> Member pos x e \<in> S \<and> S \<union> ((\<lambda>r. Member pos x r)) ` (set fs) \<in> C \<longrightarrow> S \<union> ((\<lambda>r. Member pos x r)) ` (set fs) \<in> C) \<and> 
               (\<forall> x e fs. eq_len_intersect e fs \<longrightarrow>  S \<union> ((\<lambda>r. Member pos x r)) ` (set fs) \<in> C \<longrightarrow> S \<union> {Member pos x e} \<in> C) \<and> 
-              (\<forall> x x1 x2 e e1 e2 f. con_fwd_prop e e1 e2 \<longrightarrow> EqAtom pos x (Fun f [x1, x2]) \<in> S \<and> Member pos x1 e1 \<in> S \<and> Member pos x2 e2 \<in> S \<longrightarrow> S \<union> {Member pos x e, EqAtom pos x (Fun f [x1,x2]), Member pos x1 e1, Member pos x2 e2} \<in> C) \<and> 
-              (\<forall> x x1 x2 e e1 e2 f. con_fwd_prop_elim e e1 e2 \<longrightarrow> EqAtom pos x (Fun f [x1, x2]) \<in> S \<and> Member pos x1 e1 \<in> S \<and> Member pos x2 e2 \<in> S \<longrightarrow> S \<union> {Member pos x e, Member pos x1 e1, Member pos x2 e2} \<in> C) \<and> 
-              (\<forall> S'. S' = S \<longrightarrow> S' \<in> C))\<close>
+              (\<forall> x x1 x2 e e1 e2 f. con_fwd_prop e e1 e2 \<longrightarrow> EqAtom pos x (Fun f [x1, x2]) \<in> S \<and> Member pos (Var x1) e1 \<in> S \<and> Member pos (Var x2) e2 \<in> S \<longrightarrow> S \<union> {Member pos x e, EqAtom pos x (Fun f [x1,x2]), Member pos (Var x1) e1, Member pos (Var x2) e2} \<in> C) \<and> 
+              (\<forall> x x1 x2 e e1 e2 f. con_fwd_prop_elim e e1 e2 \<longrightarrow> EqAtom pos x (Fun f [x1, x2]) \<in> S \<and> Member pos (Var x1) e1 \<in> S \<and> Member pos (Var x2) e2 \<in> S \<longrightarrow> S \<union> {Member pos x e, Member pos (Var x1) e1, Member pos (Var x2) e2} \<in> C) \<and> 
+              (\<forall> S'. S' = S \<longrightarrow> S' \<in> C))"
 
 subsection \<open>Completeness\<close>
 
+theorem TCd_consistency:
+  assumes inf_param: \<open>infinite (UNIV::'a set)\<close>
+  shows \<open>consistency {S:: string form set. \<exists>G. S = set G \<and> \<not> (\<stileturn> G)}\<close>
+  unfolding consistency_def
+proof (intro conjI allI impI notI)
+  fix S :: \<open>string form set\<close>
+  assume \<open>S \<in> {set G | G. \<not> (\<stileturn> G)}\<close> (is \<open>S \<in> ?C\<close>)
+  then obtain G :: \<open>string form list\<close>
+    where *: \<open>S = set G\<close> and \<open>\<not> (\<stileturn> G)\<close>
+    by blast
+  { 
+    assume \<open>FF \<in> S\<close>
+    then show False
+      using * Basic Order \<open>\<not> (\<stileturn> G)\<close> by auto 
+  }
+  {
+    fix A B 
+    assume \<open>Con A B \<in> S\<close>
+    then show "S \<union> {A, B} \<in> {set G |G. \<not> (\<stileturn> G)}"
+      using * \<open>\<not> (\<stileturn> G)\<close> AlphaCon Order apply auto 
+      by (metis insert_absorb list.simps(15))
+  }
+  {
+    fix A B 
+    assume \<open>form.Neg (Dis A B) \<in> S\<close>
+    then show \<open> S \<union> {form.Neg A, form.Neg B} \<in> {set G |G. \<not> (\<stileturn> G)}\<close>
+      using * \<open>\<not> (\<stileturn> G)\<close> Order AlphaNegOr apply auto
+      by (metis insert_absorb list.simps(15))
+  }
+  {
+    fix A B 
+    assume \<open>Dis A B \<in> S\<close>
+    then show \<open>S \<union> {A} \<in> {set G |G. \<not> (\<stileturn> G)} \<or> S \<union> {B} \<in> {set G |G. \<not> (\<stileturn> G)}\<close>
+      using * \<open>\<not> (\<stileturn> G)\<close> Order AlphaOr apply auto 
+      by (metis insert_absorb list.simps(15))
+  }
+  {
+    fix A B 
+    assume \<open>form.Neg (Con A B) \<in> S\<close>
+    then show \<open>S \<union> {form.Neg A} \<in> {set G |G. \<not> (\<stileturn> G)} \<or> S \<union> {form.Neg B} \<in> {set G |G. \<not> (\<stileturn> G)}\<close>
+      using * \<open>\<not> (\<stileturn> G)\<close> Order AlphaNegAnd apply auto 
+      by (metis insert_absorb list.simps(15))
+  }
+  {
+    fix A
+    assume \<open>form.Neg (form.Neg A) \<in> S\<close>
+    then show \<open>S \<union> {A} \<in> {set G |G. \<not> (\<stileturn> G)}\<close>
+      using * \<open>\<not> (\<stileturn> G)\<close> Order AlphaNegNeg apply auto 
+      by (metis insert_absorb list.simps(15))
+  }
+  {
+    fix x e ec 
+    assume \<open>regexp_compl e ec\<close> and \<open> Member neg x e \<in> S\<close>
+    then show \<open>S \<union> {Member pos x ec} \<in> {set G |G. \<not> (\<stileturn> G)}\<close>
+      using * \<open>\<not> (\<stileturn> G)\<close> Order NotMember apply auto
+      by (metis insert_absorb list.simps(15))
+  }
+  {
+    fix x y f xs 
+    assume \<open>EqAtom neg x (Fun f xs) \<in> S\<close>
+    then show \<open>S \<union> {EqAtom neg x y, EqAtom pos y (Fun f xs)} \<in> {set G |G. \<not> (\<stileturn> G)}\<close>
+      using * \<open>\<not> (\<stileturn> G)\<close> Order NotEq apply auto
+      by (metis insert_absorb list.simps(15))
+  }
+
+
+
+
+
+
 theorem SC_completeness':
   fixes p :: \<open>string form\<close>
-  assumes  mod: \<open>\<forall>e f. list_all (eval e f) ps \<longrightarrow> eval e f p\<close>
+  assumes  mod: \<open>\<forall>e f. list_all (eval e f) ps \<Longrightarrow> eval e f p\<close>
   shows \<open>SC_proof ps p\<close>
   apply(rule ccontr)
   sorry
